committing to share

disk-betree/BlockInterface.dfy
@@ -136,36 +136,38 @@ abstract module BlockInterface {
 
   /////////// Some helper facts
 
-  // function AllocatedReferences(steps: seq<Step>) : iset<Reference>
-  //   requires ValidTransaction(steps)
-  // {
-  //   //iset ref | (exists i :: 0 <= i < |steps| && steps[i].AllocStep? && steps[i].ref == ref)
-  //   if |steps| == 0 then iset{}
-  //   else
-  //     (if steps[0].AllocStep? then iset{steps[0].ref} else iset{}) + AllocatedReferences(steps[1..])
-  // }
+  function AllocatedReferences(steps: seq<Step>) : iset<Reference>
+    requires ValidTransaction(steps)
+  {
+    //iset ref | (exists i :: 0 <= i < |steps| && steps[i].AllocStep? && steps[i].ref == ref)
+    if |steps| == 0 then iset{}
+    else
+      (if steps[0].AllocStep? then iset{steps[0].ref} else iset{}) + AllocatedReferences(steps[1..])
+  }
   
-  // lemma PostTransactionView(k: Constants, s: Variables, s': Variables, steps: seq<Step>)
-  //   requires NextStep(k, s, s', TransactionStep(steps))
-  //   requires ValidTransaction(steps)
-  //   ensures s'.view.Keys == s.view.Keys + AllocatedReferences(steps)
-  // {
-  //   if |steps| == 0 {
-  //   } else {
-  //     var path: seq<Variables> :| IsStatePath(k, s, s', steps, path);
-  //     if steps[0].WriteStep? {
-  //       assert steps[0].ref in path[0].view;
-  //       assert path[1].view.Keys == path[0].view.Keys;
-  //     } else {
-  //       assert path[1].view.Keys == s.view.Keys + AllocatedReferences([steps[0]]);
-  //     }
-  //   }
-  // }
+  lemma PostTransactionView(k: Constants, s: Variables, s': Variables, steps: seq<Step>)
+    requires NextStep(k, s, s', TransactionStep(steps))
+    requires ValidTransaction(steps)
+    ensures s'.view.Keys == s.view.Keys + AllocatedReferences(steps)
+  {
+    if |steps| == 0 {
+    } else {
+      var path: seq<Variables> :| IsStatePath(k, s, s', steps, path);
+      if steps[0].WriteStep? {
+        assert steps[0].ref in path[0].view;
+        assert path[1].view.Keys == path[0].view.Keys;
+      } else {
+        assert steps[0].ref !in path[0].view;
+        assert path[1].view.Keys == s.view.Keys + AllocatedReferences([steps[0]]);
+      }
+    }
+  }
     
   
   /////////// Invariants
 
   predicate Inv(k: Constants, s: Variables) {
+    && Root(k) in s.view // Redundant? (yes, but can we delete it?)
     && ViewAndRefGraphAreConsistent(k, s)
     && RefGraphIsClosed(k, s)
     && LiveDataAvailable(k, s)
@@ -207,6 +209,7 @@ abstract module BlockInterface {
     requires GC(k, s, s', refs)
     ensures Inv(k, s')
   {
+    assert LookupIsValid(k, s, [Root(k)]);
   }
 
   lemma NextStepPreservesInv(k: Constants, s: Variables, s': Variables, step: Step)
